remove name from op[

SSASlow.lean
@@ -20,7 +20,6 @@ def Var.unit : Var := { name := "_", kind := .kind_a }
 
 inductive Op: Type where
 | op (ret : Var)
-   (name : String)
    (arg : List Var): Op 
 
 -- Lean type that corresponds to kind.
@@ -45,8 +44,8 @@ inductive Op' where
 
 def Op.denote 
  (sem: (o: Op') → Val) : Op  → Val 
-| .op _ name _ => 
-    let op' : Op' := .mk name [⟨.kind_a, 0⟩] 
+| .op _ _ => 
+    let op' : Op' := .mk "x" [⟨.kind_a, 0⟩] 
     let out := sem op'
     { kind := out.kind, val := out.val : Val }
 
@@ -65,7 +64,7 @@ def sem: (o: Op') → Val
 | _ => ⟨.kind_a, 0⟩
 
 set_option maxHeartbeats 200000
-theorem Fail: runOp sem (Op.op  Var.unit "float" [Var.unit]) = output  := by {
+theorem Fail: runOp sem (Op.op Var.unit [Var.unit]) = output  := by {
   -- ERROR:
   -- tactic 'simp' failed, nested error:
   -- (deterministic) timeout at 'whnf', maximum number of heartbeats (200000) has been reached (use 'set_option maxHeartbeats <num>' to set the limit)
